comment linked lists and queue

Examples/llist.v
@@ -8,7 +8,9 @@ Unset Strict Implicit.
 Unset Printing Implicit Defensive.
 Obligation Tactic := auto.
 
-(* linked lists, storing a value and next pointer in consecutive locations *)
+(* Linked lists, storing a value and next pointer in consecutive locations. *)
+(* We start with a more general "segment" definition, where the last node's *)
+(* next pointer is an arbitrary q *)
 
 Fixpoint lseg {A} (p q : ptr) (xs : seq A) :=
   if xs is hd::tl then
@@ -16,10 +18,14 @@ Fixpoint lseg {A} (p q : ptr) (xs : seq A) :=
        h = p :-> hd \+ (p .+ 1 :-> r \+ h') /\ h' \In lseg r q tl]
   else [Pred h | p = q /\ h = Unit].
 
+Definition EmptyList : exn := exn_from_nat 15.
+
 Section LSeg.
 Variable A : Type.
 
-Lemma lseg_add_last (xs : seq A) x p r h :
+(* appending a value to the list segment *)
+
+Lemma lseg_rcons (xs : seq A) x p r h :
         h \In lseg p r (rcons xs x) <->
         exists q h', h = h' \+ (q :-> x \+ q .+ 1 :-> r) /\ h' \In lseg p q xs.
 Proof.
@@ -33,40 +39,51 @@ exists z, (h2 \+ q :-> y \+ q .+ 1 :-> r).
 by rewrite -!joinA; split=>//; apply/IH; eauto.
 Qed.
 
+(* null pointer represents an empty segment *)
+
 Lemma lseg_null (xs : seq A) q h :
-         valid h -> h \In lseg null q xs ->
-         [/\ q = null, xs = [::] & h = Unit].
+        valid h -> h \In lseg null q xs ->
+        [/\ q = null, xs = [::] & h = Unit].
 Proof.
 case: xs=>[|x xs] D /= H; first by case: H=><- ->.
 case: H D=>r [h'][->] _; rewrite validPtUn; hhauto.
 Qed.
 
-Lemma lseg_neq (xs : seq A) p q h :
-        p != q -> h \In lseg p q xs ->
-        exists x r h',
-         [/\ xs = x :: behead xs,
-             p :-> x \+ (p .+ 1 :-> r \+ h') = h &
-             h' \In lseg r q (behead xs)].
-Proof.
-case: xs=>[|x xs] /= H []; last by move=>y [h'][->] H1; hhauto.
-by move=>E; rewrite E eq_refl in H.
-Qed.
+(* empty heap represents an empty segment *)
 
 Lemma lseg_empty (xs : seq A) p q : Unit \In lseg p q xs -> p = q /\ xs = [::].
 Proof.
 by case: xs=>[|x xs][] // r [h][/esym/join0E][/unitbE]; rewrite /heap_pts ptsU um_unitbU.
 Qed.
 
+(* reformulation of the specification *)
+
 Lemma lseg_case (xs : seq A) p q h :
         h \In lseg p q xs ->
         [/\ p = q, xs = [::] & h = Unit] \/
         exists x r h',
-          [/\ xs = x :: behead xs, h = p :-> x \+ (p .+ 1 :-> r \+ h') &
+          [/\ xs = x :: behead xs,
+              h = p :-> x \+ (p .+ 1 :-> r \+ h') &
               h' \In lseg r q (behead xs)].
 Proof.
 case: xs=>[|x xs] /=; first by case=>->->; left.
 by case=>r [h'][->] H; right; hhauto.
 Qed.
+
+(* non-trivial segment represents a non-empty list *)
+
+Corollary lseg_neq (xs : seq A) p q h :
+        p != q -> h \In lseg p q xs ->
+        exists x r h',
+         [/\ xs = x :: behead xs,
+             h = p :-> x \+ (p .+ 1 :-> r \+ h') &
+             h' \In lseg r q (behead xs)].
+Proof.
+move=>H /lseg_case; case=>//; case=>E.
+by rewrite E eq_refl in H.
+Qed.
+
+(* splitting the list corresponds to splitting the heap *)
 
 Lemma lseg_cat (xs ys : seq A) p q h :
         h \In lseg p q (xs++ys) <->
@@ -86,38 +103,42 @@ Qed.
 
 End LSeg.
 
-(* Special case when q = null *)
+(* Special case when q = null, i.e. the list is self-contained *)
 Definition lseq {A} p (xs : seq A) := lseg p null xs.
 
 Section LList.
-Variable A : Type.
+Variable (A : Type).
 
-Lemma lseq_null (xs : seq A) h : valid h -> h \In lseq null xs -> xs = [::] /\ h = Unit.
+(* specializing the null and neq lemmas *)
+
+Lemma lseq_null (xs : seq A) h :
+        valid h -> h \In lseq null xs -> xs = [::] /\ h = Unit.
 Proof. by move=>D; case/(lseg_null D)=>_ ->. Qed.
 
 Lemma lseq_pos (xs : seq A) p h :
         p != null -> h \In lseq p xs ->
         exists x r h',
           [/\ xs = x :: behead xs,
-              p :-> x \+ (p .+ 1 :-> r \+ h') = h & h' \In lseq r (behead xs)].
+              h = p :-> x \+ (p .+ 1 :-> r \+ h') &
+              h' \In lseq r (behead xs)].
 Proof. by apply: lseg_neq. Qed.
+
+(* a valid heap cannot match two different specs *)
 
 Lemma lseq_func (l1 l2 : seq A) p h :
         valid h -> h \In lseq p l1 -> h \In lseq p l2 -> l1 = l2.
 Proof.
 elim: l1 l2 p h => [|x1 xt IH] /= l2 p h V.
 - by case=>->->; case/lseq_null.
-case=>q1 /=[h1][E] H; rewrite {}E in H V *.
-case/(lseq_pos (defPt_nullO V))=>x2 [q2][h2][->] /= /esym.
+case=>q1 /= [h1][E] H; rewrite {}E in H V *.
+case/(lseq_pos (defPt_nullO V))=>x2 [q2][h2][->] /=.
 do 2![case/(cancel V)=>/dynE/jmE<-{}V].
 by move=><- /(IH (behead l2) _ _ V H)=>->.
 Qed.
 
 (* main methods *)
 
-Definition EmptyList : exn := exn_from_nat 100.
-
-(* prepending *)
+(* prepending a value *)
 
 Program Definition insert p (x : A) :
   {l}, STsep (lseq p l, [vfun p' => lseq p' (x::l)]) :=
@@ -125,33 +146,36 @@ Program Definition insert p (x : A) :
       q ::= x;;
       ret q).
 Next Obligation.
-move=>p x [l []] i /= H; step=>q.
-by rewrite unitR -joinA; heval.
+(* pull out ghost var + precondition, run the first step *)
+move=>p x [l][] i /= H; step=>q.
+(* run the last 2 steps, guess the final pointer and heap from the goal *)
+rewrite unitR -joinA; heval.
 Qed.
 
-(* head *)
+(* getting the head element *)
+(* an example of a partial program, doesn't modify the heap *)
 
 Program Definition head p :
   {l}, STsep (lseq p l,
               fun (y : ans A) h => h \In lseq p l /\
-                if y is Val v then l = v :: behead l
-                  else y = Exn EmptyList /\ l = [::]) :=
+                match y with Val v => l = v :: behead l
+                           | Exn e => e = EmptyList /\ l = [::] end) :=
   Do (if p == null then throw EmptyList
         else v <-- !p;
              ret v).
-Next Obligation. by []. Qed.
 Next Obligation.
-move=>p [l [] i] /= H.
-case: ifP H.
-- move/eqP=>-> H.
+(* pull out ghost + precondition, branch *)
+move=>p [l][] i /= H; case: ifP H=>[/eqP-> H|/negbT Hp].
+- (* there is no head element, abort *)
   step=>V; do!split=>//.
+  (* the only non-trivial goal is the list being empty *)
   by case/lseq_null: H.
-move/negbT=>H'; case/(lseq_pos H')=>v [r][h1][E <- H1].
-do 2![step]=>_; split=>//.
-by rewrite E /=; exists r, h1.
+(* deconstruct non-empty list, run the rest *)
+case/(lseq_pos Hp)=>v [r][h1][E {i}-> H1].
+by do 2![step]=>_; split=>//; rewrite E; hhauto.
 Qed.
 
-(* removing *)
+(* removing the head element, no-op for an empty list *)
 
 Program Definition remove p :
   {xs : seq A}, STsep (lseq p xs, [vfun p' => lseq p' (behead xs)]) :=
@@ -161,14 +185,20 @@ Program Definition remove p :
            dealloc p .+ 1;;
            ret pnext).
 Next Obligation.
-move=>p [xs []] i /= H; apply: vrfV=>V; case: ifP H=>H1.
-- by rewrite (eqP H1); case/(lseq_null V)=>->->; heval.
-case/(lseq_pos (negbT H1))=>x [q][h][->] <- /= H2.
+(* pull out ghost + precondition, branch *)
+move=>p [xs][] i /= H; case: ifP H=>[/eqP-> H|/negbT Ep].
+- (* the list must be empty *)
+  by step=>V; case/lseq_null: H=>//->->.
+(* deconstruct non-empty list, run the rest *)
+case/(lseq_pos Ep)=>x [q][h][-> {i}-> /= H1].
 by heval; rewrite 2!unitL.
 Qed.
 
-(* length *)
+(* calculating the list length *)
 
+(* the loop invariant: *)
+(* 1. heap is unchanged *)
+(* 2. total length is accumulator + the length of unprocessed list *)
 Definition lenT : Type := forall (pl : ptr * nat),
   {xs : seq A}, STsep (lseq pl.1 xs,
                       [vfun l h => l == pl.2 + length xs /\ lseq pl.1 xs h]).
@@ -181,21 +211,27 @@ Program Definition len p :
                             else pnext <-- !(p .+ 1);
                                  go (pnext, l + 1)))
       in len (p, 0)).
+(* first, the loop *)
 Next Obligation.
-move=>_ go ? p l /= _ [xs []] i /= H; apply: vrfV=>V.
-case: eqP H=>[->|/eqP Hp].
-- by case/(lseq_null V)=>->->/=; step; rewrite addn0.
-case/lseq_pos=>// x0 [r][h'][->] <- /= H1.
-step.
-apply: [gR (behead xs)] @ h'=>//= _ h2 [/eqP -> Hl] /= _.
+(* pull out ghosts+precondition, branch *)
+move=>_ go _ p l /= _ [xs][] i /= H; case: eqP H=>[->|/eqP Ep] H.
+- (* the end is reached *)
+  by step=>V; case/(lseq_null V): H=>->->/=; rewrite addn0.
+(* deconstruct non-empty list, run one step *)
+case/lseq_pos: H=>// x0 [r][h'][-> {i}-> /= H1]; step.
+(* feed a new ghost var and a subheap to run on to the recursive call *)
+apply: [gR (behead xs)]@h'=>//= _ h2 [/eqP -> Hl] /= _.
 by rewrite -addnA add1n; eauto.
 Qed.
 Next Obligation.
-by move=>p [xs []] i H; apply: [gE xs].
+(* pull out the ghost var and immediately feed it to the loop *)
+by move=>/= p [xs []] i /= H; apply: [gE xs].
 Qed.
 
-(* concatenation *)
+(* concatenation: modifies the first list, returning nothing *)
 
+(* the loop invariant: *)
+(* the first list should not be empty and not overlap the second *)
 Definition catT (p2 : ptr) : Type :=
   forall (p1 : ptr), {xs1 xs2 : seq A},
     STsep (fun h => p1 != null /\ (lseq p1 xs1 # lseq p2 xs2) h,
@@ -214,32 +250,48 @@ Program Definition concat p1 p2 :
            then ret p2
            else cat p1;;
                 ret p1).
+(* first, the loop *)
 Next Obligation.
-move=>_ p2 go q [xs1][xs2][_ /= [Hq][i1][i2]][-> H1 H2].
-case/(lseq_pos Hq): H1=>x [r][i][E <-{i1} H1]; step.
+(* pull out ghosts + preconditions *)
+move=>_ p2 go q [xs1][xs2][] _ /= [Hq][i1][i2][-> H1 H2].
+(* deconstruct the first non-empty list, branch *)
+case/(lseq_pos Hq): H1=>x [r][i][E {i1}-> H1]; step.
 case: ifP H1=>[/eqP ->{r}|/negbT N] H1.
-- do 2![step]=>V.
+- (* we've reached the last node of the first list *)
+  (* make it point to the second list *)
+  do 2![step]=>V.
+  (* the remaining heap for the first list is empty *)
   case/(lseq_null (validX V)): H1 E=>/=->->->/=.
-  by rewrite unitR -joinA; exists p2, i2.
+  (* the rest is just the second list *)
+  by rewrite unitR -joinA; eauto.
+(* bring i and i2 together for the recursive call *)
 rewrite -!joinA.
-apply: [gR (behead xs1), xs2] @ (i \+ i2)=>//=.
-- by split=>//; exists i, i2.
-by move=>_ m ??; rewrite E /=; exists r, m.
+(* feed new ghosts and subheap to it *)
+apply: [gR (behead xs1), xs2]@(i \+ i2)=>//= _.
+- (* the tail is not null so the precondition is satisfied *)
+  by split=>//; vauto.
+(* assemble the concatenation from head and tail *)
+by move=>m H _; rewrite E /=; eauto.
 Qed.
+(* next, the initial call *)
 Next Obligation.
-move=>p1 p2 [xs1][xs2][/= _ [i1][i2][-> H1 H2]].
+(* pull out ghosts + preconditions, branch *)
+move=>p1 p2 [xs1][xs2][] /= _ [i1][i2][-> H1 H2].
 case: ifP H1=>[/eqP ->|/negbT N] H1.
-- by step=>V; case/(lseq_null (validL V)): H1=>->->; rewrite unitL.
+- (* first list is empty, the result simplifies to the second list *)
+  by step=>V; case/(lseq_null (validL V)): H1=>->->; rewrite unitL.
+(* otherwise, feed everything to the loop *)
 by apply: [stepE xs1, xs2]=>[|[] //= [] m Hm]; heval.
 Qed.
 
+(* in-place reversal by pointer swinging *)
 
-(* in-place reversal *)
-
-Definition shape_rev p (s1 s2 : seq A) := [Pred h | h \In lseq p.1 s1 # lseq p.2 s2].
-
-Definition revT : Type := forall p,
-  {i done}, STsep (shape_rev p i done, [vfun y => lseq y (catrev i done)]).
+(* the loop invariant: *)
+(* 1. the processed and remaining parts should not overlap *)
+(* 2. the result is processed part + a reversal of remainder *)
+Definition revT : Type := forall (p : ptr * ptr),
+  {i done : seq A}, STsep (lseq p.1 i # lseq p.2 done,
+                          [vfun y => lseq y (catrev i done)]).
 
 Program Definition reverse p :
   {xs : seq A}, STsep (lseq p xs, [vfun p' => lseq p' (rev xs)]) :=
@@ -249,25 +301,35 @@ Program Definition reverse p :
                                  i .+ 1 ::= done;;
                                  go (next, i)))
       in reverse (p, null)).
+(* first, the loop *)
 Next Obligation.
-move=>_ go _ p done _ [x1][x2][] _ /= [i1][i2][-> H1 H2]; apply: vrfV=>V.
-case: eqP H1=>[->|E].
-- by case/(lseq_null (validL V))=>->->; rewrite unitL; step.
-case/lseq_pos=>[|xd [xn][h'][->] <- /= H1]; first by case: eqP.
+(* pull out ghosts + preconditions, branch *)
+move=>_ go _ i done _ [x1][x2][] _ /= [i1][i2][-> H1 H2].
+case: eqP H1=>[->|/eqP E] H1.
+- (* nothing left to reverse, return the accumulator *)
+  by step=>/validL V1; case/(lseq_null V1): H1=>->->/=; rewrite unitL.
+(* deconstruct non-empty remainder *)
+case/lseq_pos: H1=>// xd [xn][h'][-> {i1}-> /= H1].
+(* swing the pointer, feed shifted ghosts to recursive call *)
 do 2!step; apply: [gE (behead x1), xd::x2]=>//=.
-by rewrite !(pull h') -!joinA; vauto.
+(* rearrange the heap to match context *)
+rewrite !(pull h') -!joinA; vauto.
 Qed.
 Next Obligation.
-by move=>p [xs][/= i H]; apply: [gE xs, [::]]=>//; exists i; hhauto.
+(* pull out ghost, feed it + empty accumulator to the loop *)
+move=>p [xs][] /= i H; apply: [gE xs, [::]]=>//=; exists i; hhauto.
 Qed.
 
 Variable B : Type.
 
-(* Type of recursive map *)
+(* list mapping, an example of a higher-order function *)
+
+(* the loop invariant: *)
+(* the result is a mapped list *)
 Definition lmapT (f : A -> B) :=
   forall (p : ptr),
     {xs : seq A}, STsep (lseq p xs,
-                         fun (_ : ans unit) => lseq p (map f xs)).
+                        [vfun _ : unit => lseq p (map f xs)]).
 
 Program Definition lmap f : lmapT f :=
   Fix (fun (lmap : lmapT f) p =>
@@ -278,22 +340,17 @@ Program Definition lmap f : lmapT f :=
              nxt <-- !p .+ 1;
              lmap nxt)).
 Next Obligation.
-(* Deconstruct the precondition *)
-move=>f lmap p [xs][] h /= P; apply: vrfV=>V.
-
-(* Use if-rule *)
-case: ifP=>[X|/negbT X].
-
-(* 1. p == null ==> The list is empty. *)
-- move/eqP: X=>Z; rewrite {}Z in P *.
-  by case: (lseq_null V P)=>->->; heval.
-
-(* 2. p != null ==> The list is non-empty. *)
-case/(lseq_pos X): P=>t [nxt][h'][-> <- /= P].
-heval.
-
-(* Decompose the list predicate *)
-by apply/[gR (behead xs)] @ h'=>//= _ h2 Q V'; eauto.
+(* pull out ghost + precondition, branch *)
+move=>f lmap p [xs][] h /= H; case: ifP H=>[/eqP ->|/negbT N] H.
+- (* the list is empty *)
+  by step=>V; case/(lseq_null V): H=>->->.
+(* deconstruct non-empty list, run the rest *)
+case/(lseq_pos N): H=>t [nxt][h'][-> {h}-> /= H]; heval.
+(* feed the tail as a ghost var + subheap to recursive call *)
+by apply/[gR (behead xs)]@h'=>//= _ h2 Q V'; eauto.
 Qed.
 
 End LList.
+
+Arguments head {A} p.
+Arguments remove {A} p.
