Examples/queue.v
@@ -16,48 +16,64 @@ Section Queue.
 Variable T : Type.
 Notation queue := (queue T).
 
+(* a queue is specified as a singly-linked list split into an initial segment and a last node *)
 Definition is_queue (fr bq : ptr) (xs : seq T) :=
   if fr == null then [Pred h | [/\ bq = null, xs = [::] & h = Unit]]
   else [Pred h | exists xt x h',
-        [/\ xs = rcons xt x,
-            valid (bq :-> x \+ (bq .+ 1 :-> null \+ h')),
-                  (bq :-> x \+ (bq .+ 1 :-> null \+ h')) = h
-          & h' \In lseg fr bq xt]].
+                 [/\ xs = rcons xt x,
+                     valid (h' \+ (bq :-> x \+ bq .+ 1 :-> null)),
+                     h = h' \+ (bq :-> x \+ bq .+ 1 :-> null) &
+                     h' \In lseg fr bq xt]].
 
+(* the structure itself is just a pair of pointers to body + last node *)
+(* insertion happens at the last node, and removal at the head *)
 Definition shape (q : queue) (xs : seq T) :=
   [Pred h | exists fr bq h',
     [/\ valid (front q :-> fr \+ (back q :-> bq \+ h')),
-              (front q :-> fr \+ (back q :-> bq \+ h')) = h &
-              h' \In is_queue fr bq xs]].
+        h = front q :-> fr \+ (back q :-> bq \+ h') &
+        h' \In is_queue fr bq xs]].
+
+(* well-formed queue is a valid heap *)
+
+Lemma shapeD q xs h : h \In shape q xs -> valid h.
+Proof. by case=>h1[bq][h'] [] D ->. Qed.
+
+(* empty queue is a pair of null pointers *)
 
 Lemma is_queue_nil fr bq h :
         h \In is_queue fr bq [::] -> [/\ fr = null, bq = null & h = Unit].
 Proof.
-by rewrite /is_queue; case: eqP =>[->[->]_->| N [[|y xt]][x][h'][]].
+by rewrite /is_queue; case: eqP=>[->[-> _ ->] | _ [[|y xt][x][h'][]]].
 Qed.
 
-Lemma is_queue_add_last fr bq xt x h :
-         (exists h', [/\ valid (bq :-> x \+ (bq .+ 1 :-> null \+ h')),
-                                bq :-> x \+ (bq .+ 1 :-> null \+ h') = h &
-                                h' \In lseg fr bq xt]) ->
-         h \In is_queue fr bq (rcons xt x).
+(* restructuring the specification for combined list *)
+
+Lemma is_queue_rcons fr bq xt x h :
+         h \In is_queue fr bq (rcons xt x) <->
+         (exists h', [/\ valid (h' \+ (bq :-> x \+ bq .+ 1 :-> null)),
+                         h = h' \+ (bq :-> x \+ bq .+ 1 :-> null) &
+                         h' \In lseg fr bq xt]).
 Proof.
-rewrite /is_queue =>[[h']][D] <- H.
-case: eqP H=>[->|_ H].
-- move: D=>/[dup]/validR/validR D0 /[swap].
-  by case/lseg_null=>//->->->; rewrite validPtUn.
-by exists xt, x, h'.
+rewrite /is_queue; split.
+- case: eqP; first by move=>-> []; case: xt.
+  by move=>N [xt'][x'][h'][/rcons_inj [->->] ???]; exists h'.
+case=>h' [D -> H]; case: eqP H=>[->|_ H]; last by vauto.
+move: (D)=>/[swap]; case/(lseg_null (validL D))=>->->->.
+by rewrite unitL validPtUn.
 Qed.
+
+(* pointers should agree in a well-formed queue *)
 
 Lemma backfront fr bq xs h :
         h \In is_queue fr bq xs -> (fr == null) = (bq == null).
 Proof.
 rewrite /is_queue; case: ifP=>[E [->]_ _| E [xt][x][h'][_] D] //.
-by case: eqP D=>// ->; rewrite validPtUn.
+by case: eqP D=>// -> /validR; rewrite validPtUn.
 Qed.
 
-Lemma shapeD q xs : forall h, h \In shape q xs -> valid h. (* proper *)
-Proof. by move=>h [h1] [bq][h'] [] D <-. Qed.
+(* main methods *)
+
+(* new queue is a pair of pointers to an empty segment *)
 
 Program Definition new :
           STsep (emp, [vfun v => shape v [::]]) :=
@@ -65,21 +81,30 @@ Program Definition new :
       y <-- alloc null;
       ret (Queue T x y)).
 Next Obligation.
-move=>[] _ /= ->.
-step=>x; step=>y; step=>V.
-exists null, null, Unit.
-by rewrite !unitR in V *; rewrite joinC.
+(* run the complete program *)
+move=>[] _ /= ->; step=>x; step=>y; step=>V.
+(* massage the heap to fit the postcondition *)
+by exists null, null, Unit; rewrite !unitR /= in V *; rewrite joinC.
 Qed.
+
+(* freeing a queue, possible only when it's empty *)
 
 Program Definition free (q : queue) :
           STsep (shape q [::], [vfun _ h => h = Unit]) :=
   Do (dealloc (front q);;
       dealloc (back q)).
 Next Obligation.
-move=>q [] _ /= [fr][bq][h][/[swap]<-/[swap]].
+(* pull out ghosts and precondition *)
+move=>q [] _ /= [fr][bq][h][/[swap]->/[swap]].
+(* both pointers are null *)
 case/is_queue_nil=>->->->; rewrite unitR=>V.
+(* run the program *)
 by do 2![step]=>_; rewrite unitR.
 Qed.
+
+(* for enqueue/dequeue we manipulate the underlying segment directly *)
+
+(* enqueuing is adding a node at the end *)
 
 Program Definition enq (q : queue) (x : T) :
   {xs}, STsep (shape q xs,
@@ -92,33 +117,38 @@ Program Definition enq (q : queue) (x : T) :
          then front q
          else ba .+ 1) ::= next).
 Next Obligation.
-move=>q x [xs][] _ /= [fr][bq][h'][D <- H].
-step=>next; do 3!step; rewrite -(backfront H) unitR.
-case: ifP H=>Ef; rewrite /is_queue ?Ef.
-- case=>_->->; step; rewrite unitR=>V.
-  exists next, next, (next :-> x \+ next .+ 1 :-> null).
-  rewrite joinA joinC; split=>//.
-  apply: (@is_queue_add_last _ _ [::]).
-  exists Unit; rewrite unitR; split=>//.
-  by exact: (validL V).
-case=>s2[x2][i2][->] {}D <- H2.
-step; rewrite joinC !joinA=>V.
-exists fr, next, (bq :-> x2 \+ bq .+ 1 :-> next \+ i2 \+ next :-> x \+ next .+ 1 :-> null).
-rewrite !joinA; split=>//.
-apply: is_queue_add_last.
-exists (bq :-> x2 \+ bq .+ 1 :-> next \+ i2).
-rewrite joinA joinC.
-rewrite -!joinA in V; move/validR/validR: V=>V.
-rewrite -2!joinA; split=>//; first by rewrite !joinA.
-by apply/lseg_add_last; exists bq, i2; rewrite joinC.
+(* pull out ghosts + precondition *)
+move=>q x [xs][] _ /= [fr][bq][h'][D -> H].
+(* create the new last node and change the back pointer *)
+step=>next; do 3!step.
+(* as the pointers agree, test the front one to reason structurally *)
+rewrite -(backfront H) unitR; case: ifP H=>Ef; rewrite /is_queue ?Ef.
+- (* the queue was empty, set the front pointer to new node *)
+  case=>_->->; step; rewrite unitR=>V.
+  (* massage the heap and restructure the goal *)
+  exists next, next, (next :-> x \+ next.+ 1 :-> null).
+  rewrite joinA joinC; split=>//; apply/(@is_queue_rcons _ _ [::]).
+  by exists Unit; rewrite unitL; split=>//; exact: (validL V).
+(* the queue wasn't empty, link the new node to the last one *)
+case=>s2[x2][i2][->] {}D -> H2; step=>V.
+(* massage the heap and simplify the goal *)
+exists fr, next, (i2 \+ bq :-> x2 \+ bq.+ 1 :-> next \+ next :-> x \+ next.+ 1 :-> null).
+split; first by apply: (validX V).
+- by rewrite joinC !joinA.
+(* the new node conforms to the queue spec *)
+apply/is_queue_rcons; exists (i2 \+ bq :-> x2 \+ bq.+ 1 :-> next).
+rewrite joinA; split=>//; first by apply: (validX V).
+(* assemble the old queue back *)
+by apply/lseg_rcons; exists bq, i2; rewrite joinA.
 Qed.
+
+(* dequeuing is removing the head node and adjusting pointers *)
 
 Program Definition deq (q : queue) :
   {xs}, STsep (shape q xs,
                fun y h => shape q (behead xs) h /\
-                 if y is Val v
-                   then xs = v :: behead xs
-                   else y = Exn EmptyQueue /\ xs = [::]) :=
+                 match y with Val v => xs = v :: behead xs
+                            | Exn e => e = EmptyQueue /\ xs = [::] end) :=
   Do (fr <-- !front q;
       if (fr : ptr) == null then throw EmptyQueue
       else
@@ -131,22 +161,32 @@ Program Definition deq (q : queue) :
           then back q ::= null;;
                ret x
         else ret x).
-Next Obligation. by []. Qed.
 Next Obligation.
-move=>q [xs][] _ /= [fr][bq][h][D <- H].
+(* pull out ghosts + precondition *)
+move=>q [xs][] _ /= [fr][bq][h][D -> H].
+(* read the list, branch *)
 step; case: ifP H=>Ef; rewrite /is_queue Ef.
-- case=>->->->/=; step=>V; split=>//.
+- (* list is empty, throw an exception *)
+  case=>->->->/=; step=>V; split=>//.
+  (* massage and simplify *)
   exists fr, null, Unit; rewrite unitR in V *; split=>//.
   by rewrite Ef.
-case=>[[|y xt]][x][h'][->] {}D {h}<- /=.
-- case=>->->; do 7!step; rewrite !unitR=>V; split=>//.
+(* deconstruct the initial segment *)
+case=>[[|y xt]][x][h'][->] {}D {h}-> /=.
+- (* segment is empty, so dequeuing returns the last node *)
+  case=>->->; do 7!step; rewrite !unitR=>V; split=>//.
   by exists null, null, Unit; rewrite unitR.
+(* segment is non-empty, run up to the branching point *)
 case=>next [h2][->] H; do 5!step; rewrite !unitL.
 case: ifP H=>[/eqP ->|N] H.
-- do 2![step]=>V2.
-  by case/(lseg_null (validX V2)): H D=>/=->.
-step=>V; split=>//; exists next, bq, (bq :-> x \+ (bq .+ 1 :-> null \+ h2)).
-by rewrite N; split=>//; exists xt, x, h2; split=>//; apply: (validX V).
+- (* null pointer is in the middle of the segment *)
+  do 2![step]=>V2.
+  (* this contradicts heap validity *)
+  case/(lseg_null (validX V2)): H D=>/=-> _ _ /validR.
+  by rewrite validPtUn.
+(* return the segment head and simplify *)
+step=>V; split=>//; exists next, bq, (h2 \+ (bq :-> x \+ bq .+ 1 :-> null)).
+by rewrite N; split=>//; vauto; apply: (validX V).
 Qed.
 
 End Queue.
